CollapsingTowers.lean
@@ -1,4 +1,2 @@
 -- This module serves as the root of the `CollapsingTowers` library.
 -- Import modules here that should be built as part of the library.
-import CollapsingTowers.TwoLevelFull.Soundness
-import CollapsingTowers.TwoLevelFull.Examples.Defs
