CollapsingTowers/TwoLevelBasic/LogicalEquiv/Transitive.lean
@@ -1,4 +1,4 @@
-import CollapsingTowers.TwoLevelBasic.LogicEquiv.Symmetry
+import CollapsingTowers.TwoLevelBasic.LogicalEquiv.Symmetry
 
 -- (v₀, v₁) ∈ 𝓥⟦τ⟧ → (v₁, v₂) ∈ 𝓥⟦τ⟧ → (v₀, v₂) ∈ 𝓥⟦τ⟧
 -- ———————————————————————————————————————————————————
@@ -6,24 +6,24 @@ import CollapsingTowers.TwoLevelBasic.LogicEquiv.Symmetry
 lemma value_trans_impl_expr_trans :
   ∀ τ,
     (∀ v₀ v₁ v₂,
-      logic_equiv_value v₀ v₁ τ →
-      logic_equiv_value v₁ v₂ τ →
-      logic_equiv_value v₀ v₂ τ) →
+      log_equiv_value v₀ v₁ τ →
+      log_equiv_value v₁ v₂ τ →
+      log_equiv_value v₀ v₂ τ) →
     (∀ e₀ e₁ e₂,
-      logic_equiv_expr e₀ e₁ τ →
-      logic_equiv_expr e₁ e₂ τ →
-      logic_equiv_expr e₀ e₂ τ) :=
+      log_equiv_expr e₀ e₁ τ →
+      log_equiv_expr e₁ e₂ τ →
+      log_equiv_expr e₀ e₂ τ) :=
   by
   intros τ Hsem_value_trans e₀ e₁ e₂ Hsem_expr₀ Hsem_expr₁
-  simp only [logic_equiv_expr] at Hsem_expr₀ Hsem_expr₁
+  simp only [log_equiv_expr] at Hsem_expr₀ Hsem_expr₁
   have ⟨v₀, v₁, Hstepv₀, Hstepv₁, Hsem_value₀⟩ := Hsem_expr₀
-  have ⟨Hvalue₀, Hvalue₁⟩ := logic_equiv_value.syntactic_value _ _ _ Hsem_value₀
+  have ⟨Hvalue₀, Hvalue₁⟩ := log_equiv_value.syntactic_value _ _ _ Hsem_value₀
   have ⟨v₂, v₃, Hstepv₂, Hstepv₃, Hsem_value₁⟩ := Hsem_expr₁
-  have ⟨Hvalue₂, Hvalue₃⟩ := logic_equiv_value.syntactic_value _ _ _ Hsem_value₁
+  have ⟨Hvalue₂, Hvalue₃⟩ := log_equiv_value.syntactic_value _ _ _ Hsem_value₁
   have Hstepv₁ := pure_stepn_impl_stepn _ _ Hstepv₁
   have Hstepv₂ := pure_stepn_impl_stepn _ _ Hstepv₂
   rw [← unique_normal_forms _ _ _ Hstepv₁ Hstepv₂ Hvalue₁ Hvalue₂] at Hsem_value₁
-  simp only [logic_equiv_expr]
+  simp only [log_equiv_expr]
   exists v₀, v₃
   constructor; apply Hstepv₀
   constructor; apply Hstepv₃
@@ -34,11 +34,11 @@ lemma value_trans_impl_expr_trans :
 -- (v₁, v₂) ∈ 𝓥⟦τ⟧
 -- ———————————————
 -- (v₀, v₂) ∈ 𝓥⟦τ⟧
-lemma logic_equiv_value.trans :
+lemma log_equiv_value.trans :
   ∀ v₀ v₁ v₂ τ,
-    logic_equiv_value v₀ v₁ τ →
-    logic_equiv_value v₁ v₂ τ →
-    logic_equiv_value v₀ v₂ τ :=
+    log_equiv_value v₀ v₁ τ →
+    log_equiv_value v₁ v₂ τ →
+    log_equiv_value v₀ v₂ τ :=
   by
   intros v₀ v₁ v₂ τ Hsem_value₀ Hsem_value₁
   induction τ generalizing v₀ v₁ v₂
@@ -54,17 +54,17 @@ lemma logic_equiv_value.trans :
     case lam e₂ =>
     cases φ
     case pure =>
-      simp only [logic_equiv_value] at Hsem_value₀ Hsem_value₁
+      simp only [log_equiv_value] at Hsem_value₀ Hsem_value₁
       have ⟨Hwf₀, Hwf₁, Hsem_value_lam₀⟩ := Hsem_value₀
       have ⟨Hwf₁, Hwf₂, Hsem_value_lam₁⟩ := Hsem_value₁
-      simp only [logic_equiv_value]
+      simp only [log_equiv_value]
       constructor; apply Hwf₀
       constructor; apply Hwf₂
       intros v₀ v₁ Hsem_value
       apply value_trans_impl_expr_trans; apply IH𝕓
       apply Hsem_value_lam₀; apply Hsem_value
       apply Hsem_value_lam₁; apply IH𝕒
-      apply logic_equiv_value.symm; apply Hsem_value; apply Hsem_value
+      apply log_equiv_value.symm; apply Hsem_value; apply Hsem_value
     case reify => simp at Hsem_value₀
   case fragment => simp at Hsem_value₀
   case rep => simp at Hsem_value₀
@@ -73,37 +73,37 @@ lemma logic_equiv_value.trans :
 -- (e₁, e₂) ∈ 𝓔⟦τ⟧
 -- ———————————————
 -- (e₀, e₂) ∈ 𝓔⟦τ⟧
-lemma logic_equiv_expr.trans :
+lemma log_equiv_expr.trans :
   ∀ e₀ e₁ e₂ τ,
-    logic_equiv_expr e₀ e₁ τ →
-    logic_equiv_expr e₁ e₂ τ →
-    logic_equiv_expr e₀ e₂ τ :=
+    log_equiv_expr e₀ e₁ τ →
+    log_equiv_expr e₁ e₂ τ →
+    log_equiv_expr e₀ e₂ τ :=
   by
   intros e₀ e₁ e₂ τ
   apply value_trans_impl_expr_trans
   intros v₀ v₁ v₂
-  apply logic_equiv_value.trans
+  apply log_equiv_value.trans
 
 -- (γ₀, γ₁) ∈ 𝓖⟦Γ⟧
 -- (γ₁, γ₂) ∈ 𝓖⟦Γ⟧
 -- ———————————————
 -- (γ₀, γ₂) ∈ 𝓖⟦Γ⟧
-lemma logic_equiv_env.trans :
+lemma log_equiv_env.trans :
   ∀ γ₀ γ₁ γ₂ Γ,
-    logic_equiv_env γ₀ γ₁ Γ →
-    logic_equiv_env γ₁ γ₂ Γ →
-    logic_equiv_env γ₀ γ₂ Γ :=
+    log_equiv_env γ₀ γ₁ Γ →
+    log_equiv_env γ₁ γ₂ Γ →
+    log_equiv_env γ₀ γ₂ Γ :=
   by
   intros γ₀ γ₁ γ₂ Γ HsemΓ₀ HsemΓ₁
   induction HsemΓ₀ generalizing γ₂
   case nil =>
     cases HsemΓ₁
-    apply logic_equiv_env.nil
+    apply log_equiv_env.nil
   case cons Hsem_value₀ _ IH =>
     cases HsemΓ₁
     case cons Hsem_value₁ _ =>
-    apply logic_equiv_env.cons
-    apply logic_equiv_value.trans
+    apply log_equiv_env.cons
+    apply log_equiv_value.trans
     apply Hsem_value₀; apply Hsem_value₁
     apply IH; assumption
 
@@ -111,21 +111,21 @@ lemma logic_equiv_env.trans :
 -- Γ ⊧ e₁ ≈ e₂ : τ
 -- ———————————————
 -- Γ ⊧ e₀ ≈ e₂ : τ
-theorem logic_equiv_typing.trans :
+theorem log_equiv_typing.trans :
   ∀ Γ e₀ e₁ e₂ τ,
-    logic_equiv_typing Γ e₀ e₁ τ →
-    logic_equiv_typing Γ e₁ e₂ τ →
-    logic_equiv_typing Γ e₀ e₂ τ :=
+    log_equiv_typing Γ e₀ e₁ τ →
+    log_equiv_typing Γ e₁ e₂ τ →
+    log_equiv_typing Γ e₀ e₂ τ :=
   by
   intros Γ e₀ e₁ e₂ τ Hsem₀ Hsem₁
-  rw [logic_equiv_typing] at Hsem₀ Hsem₁
-  rw [logic_equiv_typing]
+  rw [log_equiv_typing] at Hsem₀ Hsem₁
+  rw [log_equiv_typing]
   have ⟨Hwf₀, Hwf₁, Hsem₀⟩ := Hsem₀
   have ⟨Hwf₁, Hwf₂, Hsem₁⟩ := Hsem₁
   constructor; apply Hwf₀
   constructor; apply Hwf₂
   intros γ₀ γ₁ HsemΓ
-  apply logic_equiv_expr.trans
+  apply log_equiv_expr.trans
   apply Hsem₀; apply HsemΓ
-  apply Hsem₁; apply logic_equiv_env.trans
-  apply logic_equiv_env.symm; apply HsemΓ; apply HsemΓ
+  apply Hsem₁; apply log_equiv_env.trans
+  apply log_equiv_env.symm; apply HsemΓ; apply HsemΓ
